proof/old_system/uni/algo_worklist/prop_rename.v
@@ -17,6 +17,70 @@ Open Scope aworklist_scope.
 #[local] Hint Rewrite awl_to_aenv_cons awl_to_aenv_app: core.
 #[local] Hint Rewrite dom_app dom_cons : core.
 
+
+Fixpoint rename_tvar_in_aworklist (X' X:typvar) (Γ:aworklist) {struct Γ} : aworklist :=
+  match Γ with
+  | aworklist_empty => aworklist_empty
+  | (aworklist_consvar Γ' x b) => aworklist_consvar (rename_tvar_in_aworklist X' X Γ') x (subst_tvar_in_abind (typ_var_f X') X b)
+  | (aworklist_constvar Γ' X0 b) => aworklist_constvar (rename_tvar_in_aworklist X' X Γ') (if X0 == X then X' else X0) (subst_tvar_in_abind (typ_var_f X') X b)
+  | (aworklist_conswork Γ' w) => aworklist_conswork (rename_tvar_in_aworklist X' X Γ') (subst_tvar_in_work (typ_var_f X') X w)
+end.
+
+Fixpoint rename_var_in_aworklist (x' x:expvar) (Γ:aworklist) {struct Γ} : aworklist :=
+  match Γ with
+  | aworklist_empty => aworklist_empty
+  | (aworklist_consvar Γ' x0 b) => aworklist_consvar (rename_var_in_aworklist x' x Γ')  (if x0 == x then x' else x0) b
+  | (aworklist_constvar Γ' X b) => aworklist_constvar (rename_var_in_aworklist x' x Γ') X b
+  | (aworklist_conswork Γ' w) => aworklist_conswork (rename_var_in_aworklist x' x Γ') (subst_var_in_work (exp_var_f x') x w)
+  end.
+
+
+(* a group of rename lemmas for tvar *)
+Lemma rename_tvar_in_aworklist_bind_same : forall Γ X1 X2 X' b,
+  ⊢ᵃʷ Γ ->
+  X' `notin` ftvar_in_aworklist' Γ ->
+  binds X1 b (awl_to_aenv Γ) ->
+  (~ exists A, b = abind_var_typ A) ->
+  binds (if X1 == X2 then X' else X1) b
+    (awl_to_aenv (rename_tvar_in_aworklist X' X2 Γ)).
+Proof with solve_false.
+  intros. induction Γ; simpl in *; auto.
+  - dependent destruction H. destruct_eq_atom.
+    + inversion H3.
+      * dependent destruction H5...
+      * apply binds_cons; auto.
+    + inversion H3.
+      * dependent destruction H5...
+      * apply binds_cons; auto.
+  - dependent destruction H; destruct_eq_atom; subst;
+    try solve constructor; inversion H2; try dependent destruction H4; try solve [apply binds_cons; auto]...
+    all: try solve [simpl; constructor; auto].
+  - destruct_eq_atom; dependent destruction H; auto.
+Qed.
+
+Corollary rename_tvar_in_aworklist_bind_same_neq : forall Γ X1 X2 X' b,
+  ⊢ᵃʷ Γ ->
+  X1 <> X2 ->
+  X' `notin` ftvar_in_aworklist' Γ ->
+  binds X1 b (awl_to_aenv Γ) ->
+  (~ exists A, b = abind_var_typ A) ->
+  binds X1 b (awl_to_aenv (rename_tvar_in_aworklist X' X2 Γ)).
+Proof.
+  intros. eapply rename_tvar_in_aworklist_bind_same with (X2:=X2) in H1; eauto.
+  destruct_eq_atom; auto.
+Qed.
+
+Corollary rename_tvar_in_aworklist_bind_same_eq : forall Γ X X' b,
+  ⊢ᵃʷ Γ ->
+  X' `notin` ftvar_in_aworklist' Γ ->
+  binds X b (awl_to_aenv Γ) ->
+  (~ exists A, b = abind_var_typ A) ->
+  binds (X') b (awl_to_aenv (rename_tvar_in_aworklist X' X Γ)).
+Proof with solve_false.
+  intros. eapply rename_tvar_in_aworklist_bind_same with (X2:=X) in H1; eauto...
+  destruct_eq_atom; auto.
+Qed.
+
 Lemma awl_app_rename_tvar_comm : forall Γ1 Γ2 X X',
   awl_app (rename_tvar_in_aworklist X' X Γ2) (rename_tvar_in_aworklist X' X Γ1) =
   rename_tvar_in_aworklist X' X (awl_app Γ2 Γ1).
@@ -631,32 +695,223 @@ Proof.
     apply rename_tvar_in_aworklist_bind_same_neq; eauto. solve_false. 
 Qed.
 
+(* Lemma awl_binds_atvar_to_env : forall Γ X X' b,
+  b = □ \/ b = ■ \/ b = ⬒ ->
+  ⊢ᵃʷ Γ ->
+  binds X b (awl_to_aenv Γ) ->
+  exists Σ1 Σ2, ⌊ Γ ⌋ᵃ = (Σ2 ++ (X, b) :: Σ1) /\ 
+               ⌊ rename_tvar_in_aworklist X' X Γ ⌋ᵃ = ((map (subst_tvar_in_abind `X' X) Σ2) ++ (X', b) :: Σ1).
+Proof with eauto.
+  intros. induction H0; simpl in *; try solve [eexists; eauto].
+  - inversion H1.
+  - destruct_binds.
+    + destruct H. inversion H. destruct H. inversion H. inversion H.
+    + apply IHa_wf_wl in H5...
+      destruct H5 as [Σ1 [Σ2 [Heq Hrenameeq]]].
+      exists Σ1 ((x, abind_var_typ A) :: Σ2). split; auto.
+      * simpl. rewrite Heq. auto.
+      * simpl. rewrite Hrenameeq. auto.
+  - destruct_binds; destruct_eq_atom.
+    + exists (⌊ Γ ⌋ᵃ), (@nil (atom * abind)). 
+      split; auto. simpl.
+      rewrite rename_tvar_in_aworklist_fresh_eq; auto.
+      rewrite ftvar_in_aworklist_upper; auto.
+    + apply binds_dom_contradiction in H4... contradiction. 
+    + apply IHa_wf_wl in H4...
+      destruct H4 as [Σ1 [Σ2 [Heq Hrenameeq]]].
+      exists Σ1 ((X0, □) :: Σ2). split; auto.
+      * simpl. rewrite Heq. auto.
+      * simpl. rewrite Hrenameeq. auto.
+  - destruct_binds; destruct_eq_atom.
+    + exists (⌊ Γ ⌋ᵃ), (@nil (atom * abind)). 
+      split; auto. simpl.
+      rewrite rename_tvar_in_aworklist_fresh_eq; auto.
+      rewrite ftvar_in_aworklist_upper; auto.
+    + apply binds_dom_contradiction in H4... contradiction. 
+    + apply IHa_wf_wl in H4...
+      destruct H4 as [Σ1 [Σ2 [Heq Hrenameeq]]].
+      exists Σ1 ((X0, ■) :: Σ2). split; auto.
+      * simpl. rewrite Heq. auto.
+      * simpl. rewrite Hrenameeq. auto.
+  - destruct_binds; destruct_eq_atom.
+    + exists (⌊ Γ ⌋ᵃ), (@nil (atom * abind)). 
+      split; auto. simpl.
+      rewrite rename_tvar_in_aworklist_fresh_eq; auto.
+      rewrite ftvar_in_aworklist_upper; auto.
+    + apply binds_dom_contradiction in H4... contradiction. 
+    + apply IHa_wf_wl in H4...
+      destruct H4 as [Σ1 [Σ2 [Heq Hrenameeq]]].
+      exists Σ1 ((X0, ⬒) :: Σ2). split; auto.
+      * simpl. rewrite Heq. auto.
+      * simpl. rewrite Hrenameeq. auto.
+  - destruct_binds; destruct_eq_atom.
+    apply IHa_wf_wl in H1...
+Qed. *)
+
+Lemma rename_tvar_dom_upper : forall Γ X X',
+  dom (awl_to_aenv (rename_tvar_in_aworklist X' X Γ)) [<=] dom (awl_to_aenv Γ) `union` singleton X'.
+Proof.
+  intros. induction Γ; simpl; try fsetdec.
+  destruct_eq_atom; fsetdec.
+Qed.
+
+
+Lemma a_wl_rename_tvar_wf_typ : forall Γ X X' A,
+  ⊢ᵃʷ Γ ->
+  X' `notin` dom (awl_to_aenv Γ) ->
+  a_wf_typ (⌊ Γ ⌋ᵃ) A ->
+  a_wf_typ (⌊ rename_tvar_in_aworklist X' X Γ ⌋ᵃ) ({` X' ᵗ/ₜ X} A).
+Proof.
+  intros. dependent induction H1; simpl in *; eauto; destruct_eq_atom; eauto.
+  - constructor; auto.
+    apply rename_tvar_in_aworklist_bind_same_eq; eauto.
+    rewrite ftvar_in_aworklist_upper; eauto. solve_false.
+  - constructor; auto.
+    apply rename_tvar_in_aworklist_bind_same_neq; eauto.
+    rewrite ftvar_in_aworklist_upper; eauto. solve_false.
+  - apply a_wf_typ__stvar.
+    apply rename_tvar_in_aworklist_bind_same_eq; eauto.
+    rewrite ftvar_in_aworklist_upper; eauto. solve_false.
+  - apply a_wf_typ__stvar.
+    apply rename_tvar_in_aworklist_bind_same_neq; eauto.
+    rewrite ftvar_in_aworklist_upper; eauto. solve_false.
+  - apply a_wf_typ__etvar.
+    apply rename_tvar_in_aworklist_bind_same_eq; eauto.
+    rewrite ftvar_in_aworklist_upper; eauto. solve_false.
+  - apply a_wf_typ__etvar.
+    apply rename_tvar_in_aworklist_bind_same_neq; eauto.
+    rewrite ftvar_in_aworklist_upper; eauto. solve_false.
+  - inst_cofinites_for a_wf_typ__all; intros; inst_cofinites_with X0...
+    + rewrite subst_tvar_in_typ_open_typ_wrt_typ_fresh2; auto.
+      apply s_in_subst_inv; auto.
+    + rewrite subst_tvar_in_typ_open_typ_wrt_typ_fresh2; auto.
+      replace (X0 ~ □ ++ ⌊ rename_tvar_in_aworklist X' X Γ ⌋ᵃ) with  
+        (⌊ rename_tvar_in_aworklist X' X (X0 ~ᵃ □ ;ᵃ Γ) ⌋ᵃ).
+      apply H1; eauto.
+      simpl. destruct_eq_atom. auto.
+Qed.
+
+
+Lemma binds_var_typ_rename_tvar : forall x A X X' Γ,
+  ⊢ᵃʷ Γ ->
+  binds x (abind_var_typ A) (awl_to_aenv Γ) ->
+  binds x (abind_var_typ ({` X' ᵗ/ₜ X} A)) (awl_to_aenv (rename_tvar_in_aworklist X' X Γ)).
+Proof with auto.
+  intros. induction Γ.
+  - simpl in *. inversion H0.
+  - simpl in *. inversion H0.
+    + dependent destruction H1.
+      simpl. constructor...
+    + apply binds_cons...
+      dependent destruction H...
+  - simpl in *. inversion H0.
+    + dependent destruction H1.
+      inversion H.
+    + dependent destruction H; apply binds_cons...
+  - dependent destruction H. simpl in *...
+Qed.
+
+
+Lemma a_wl_rename_tvar_wf_exp : forall Γ X X' e,
+  ⊢ᵃʷ Γ ->
+  X' `notin` dom (awl_to_aenv Γ) ->
+  a_wf_exp (⌊ Γ ⌋ᵃ) e ->
+  a_wf_exp (⌊ rename_tvar_in_aworklist X' X Γ ⌋ᵃ) (subst_tvar_in_exp (typ_var_f X') X e)
+with a_wl_rename_tvar_wf_body : forall Γ X X' b,
+  ⊢ᵃʷ Γ ->
+  X' `notin` dom (awl_to_aenv Γ) ->
+  a_wf_body (⌊ Γ ⌋ᵃ) b ->
+  a_wf_body (⌊ rename_tvar_in_aworklist X' X Γ ⌋ᵃ) (subst_tvar_in_body (typ_var_f X') X b).
+Proof with eauto using a_wl_rename_tvar_wf_typ.
+  - intros. clear a_wl_rename_tvar_wf_exp. dependent induction H1; simpl in *; auto...
+    + eapply binds_var_typ_rename_tvar with (X':=X') (X:=X) in H1...
+    + inst_cofinites_for a_wf_exp__abs T:=({`X' ᵗ/ₜ X}T)...
+      intros. inst_cofinites_with x.
+      replace (x ~ abind_var_typ ({` X' ᵗ/ₜ X} T) ++ ⌊ rename_tvar_in_aworklist X' X Γ ⌋ᵃ) with  
+      (⌊ rename_tvar_in_aworklist X' X (x ~ᵃ T ;ᵃ Γ) ⌋ᵃ).
+      replace (subst_tvar_in_exp ` X' X e ᵉ^ₑ exp_var_f x) with (subst_tvar_in_exp ` X' X (e ᵉ^ₑ exp_var_f x)).
+      apply H1...
+      rewrite subst_tvar_in_exp_open_exp_wrt_exp...
+      simpl. destruct_eq_atom...
+    + inst_cofinites_for a_wf_exp__tabs; intros; inst_cofinites_with X0...
+      * rewrite subst_tvar_in_body_open_body_wrt_typ_fresh2...
+        apply s_in_b_subst_inv...
+      * rewrite subst_tvar_in_body_open_body_wrt_typ_fresh2; auto.
+        replace (X0 ~ □ ++ ⌊ rename_tvar_in_aworklist X' X Γ ⌋ᵃ) with  
+          (⌊ rename_tvar_in_aworklist X' X (X0 ~ᵃ □ ;ᵃ Γ) ⌋ᵃ).
+        apply a_wl_rename_tvar_wf_body; eauto.
+        simpl. destruct_eq_atom. auto.
+  - intros. clear a_wl_rename_tvar_wf_body. dependent destruction H1; simpl in *; auto...
+Qed.
+
+
+Lemma a_wf_exp_weaken_etvar_twice : forall x X1 X2 T e Γ,
+  x ~ abind_var_typ T ++ ⌊ Γ ⌋ᵃ ᵉ⊢ᵃ e ᵉ^ₑ exp_var_f x ->
+  (x, abind_var_typ ` X1) :: (X2, ⬒) :: (X1, ⬒) :: ⌊ Γ ⌋ᵃ ᵉ⊢ᵃ e ᵉ^ₑ exp_var_f x.
+Proof.
+  intros. apply a_wf_exp_var_binds_another_cons with (A1:=T); auto.
+  rewrite_env ((x ~ abind_var_typ T) ++ ((X2, ⬒) :: (X1 ~ ⬒)) ++ ⌊ Γ ⌋ᵃ).
+  apply a_wf_exp_weaken; auto.
+Qed.
+
+#[local] Hint Immediate  a_wf_exp_weaken_etvar_twice : core.
+
+Lemma a_wl_rename_tvar_wf_conts : forall Γ X X' cs,
+  ⊢ᵃʷ Γ ->
+  X' `notin` dom (awl_to_aenv Γ) ->
+  a_wf_conts (⌊ Γ ⌋ᵃ) cs ->
+  a_wf_conts (⌊ rename_tvar_in_aworklist X' X Γ ⌋ᵃ) (subst_tvar_in_conts (typ_var_f X') X cs)
+with a_wl_rename_tvar_wf_contd : forall Γ X X' cd,
+  ⊢ᵃʷ Γ ->
+  X' `notin` dom (awl_to_aenv Γ) ->
+  a_wf_contd (⌊ Γ ⌋ᵃ) cd ->
+  a_wf_contd (⌊ rename_tvar_in_aworklist X' X Γ ⌋ᵃ) (subst_tvar_in_contd (typ_var_f X') X cd).
+Proof with auto using a_wl_rename_tvar_wf_typ, a_wl_rename_tvar_wf_exp.
+  - intros. clear a_wl_rename_tvar_wf_conts. dependent induction H1; simpl in *; auto...
+  - intros. clear a_wl_rename_tvar_wf_contd. dependent induction H1; try repeat destruct_wf_arrow; simpl in *; auto...
+Qed.
+
+Lemma a_wl_rename_tvar_wf_work : forall Γ X X' w,
+  ⊢ᵃʷ Γ ->
+  X' `notin` dom (awl_to_aenv Γ) ->
+  a_wf_work (⌊ Γ ⌋ᵃ) w ->
+  a_wf_work (⌊ rename_tvar_in_aworklist X' X Γ ⌋ᵃ) (subst_tvar_in_work (typ_var_f X') X w).
+Proof with auto 8 using a_wl_rename_tvar_wf_typ, a_wl_rename_tvar_wf_exp, a_wl_rename_tvar_wf_conts, a_wl_rename_tvar_wf_contd.
+  intros. dependent destruction H1; try repeat destruct_wf_arrow; simpl... 
+Qed.
+  
+
 Lemma a_wf_wl_rename_tvar : forall Γ X X',
   ⊢ᵃʷ Γ ->
   X' `notin` dom (awl_to_aenv Γ) ->
   ⊢ᵃʷ (rename_tvar_in_aworklist X' X Γ).
-Proof.
+Proof with eauto.
   intros. induction H; try solve [simpl in *; eauto].
-  - simpl in *. econstructor; auto.
-    admit. admit.
-  - simpl in *. destruct (X0 == X); subst.
-    + constructor; auto.
-      rewrite rename_tvar_in_aworklist_fresh_eq; auto.
-      rewrite <- ftvar_in_aworklist_upper in H; auto.
-    + constructor; auto. admit.
-  - simpl in *. destruct (X0 == X); subst.
-    + constructor; auto.
-      rewrite rename_tvar_in_aworklist_fresh_eq; auto.
-      rewrite <- ftvar_in_aworklist_upper in H; auto.
-    + constructor; auto. admit.
-  - simpl in *. destruct (X0 == X); subst.
-    + constructor; auto.
-      rewrite rename_tvar_in_aworklist_fresh_eq; auto.
-      rewrite <- ftvar_in_aworklist_upper in H; auto.
-    + constructor; auto. admit.
+  - simpl in *.  destruct_binds.
+    + econstructor; auto.
+      rewrite rename_tvar_dom_upper. fsetdec.
+      apply a_wl_rename_tvar_wf_typ...
+  - simpl in *. destruct_binds; destruct_eq_atom. 
+    + rewrite rename_tvar_in_aworklist_fresh_eq; auto.
+      rewrite <- ftvar_in_aworklist_upper in H; auto...
+    + assert (X' ∉ dom (⌊ Γ ⌋ᵃ)) by auto.  
+      apply IHa_wf_wl in H2. constructor; auto.
+      rewrite rename_tvar_dom_upper; auto.
+  - simpl in *. destruct_binds; destruct_eq_atom. 
+    + rewrite rename_tvar_in_aworklist_fresh_eq; auto.
+      rewrite <- ftvar_in_aworklist_upper in H; auto...
+    + assert (X' ∉ dom (⌊ Γ ⌋ᵃ)) by auto.  
+      apply IHa_wf_wl in H2. constructor; auto.
+      rewrite rename_tvar_dom_upper; auto.
+  - simpl in *. destruct_binds; destruct_eq_atom. 
+    + rewrite rename_tvar_in_aworklist_fresh_eq; auto.
+      rewrite <- ftvar_in_aworklist_upper in H; auto...
+    + assert (X' ∉ dom (⌊ Γ ⌋ᵃ)) by auto.  
+      apply IHa_wf_wl in H2. constructor; auto.
+      rewrite rename_tvar_dom_upper; auto.
   - simpl in *. constructor; auto.
-    admit.
-Admitted.
+    apply a_wl_rename_tvar_wf_work...
+Qed.
 
 
 Lemma apply_conts_rename_tvar : forall cs A w X X',
@@ -739,6 +994,8 @@ Ltac fold_subst :=
   match goal with
   | _ : _ |- context [typ_arrow ({` ?X' ᵗ/ₜ ?X} ?A1) ({` ?X' ᵗ/ₜ ?X} ?A2)] => 
     replace (typ_arrow ({` X' ᵗ/ₜ X} A1) ({` X' ᵗ/ₜ X} A2)) with ({` X' ᵗ/ₜ X} (typ_arrow A1 A2)) by auto
+  | H : context [typ_arrow ({` ?X' ᵗ/ₜ ?X} ?A1) ({` ?X' ᵗ/ₜ ?X} ?A2)] |- _ => 
+    replace (typ_arrow ({` X' ᵗ/ₜ X} A1) ({` X' ᵗ/ₜ X} A2)) with ({` X' ᵗ/ₜ X} (typ_arrow A1 A2)) in H by auto
   end.
 
 
@@ -812,8 +1069,7 @@ Proof with eauto; solve_false.
       destruct_a_wf_wl; auto.
     + destruct_a_wf_wl.
       fold_subst. apply a_mono_typ_false_rename; simpl; eauto.
-    + intros. replace (typ_arrow ({` X' ᵗ/ₜ X} A1) ({` X' ᵗ/ₜ X} A2)) with ({` X' ᵗ/ₜ X} (typ_arrow A1 A2)) in H7...  
-      eapply s_in_subst in H7...
+    + intros. fold_subst. eapply s_in_subst in H7...
     + intros. simpl in *.
       apply worklist_subst_rename_tvar with (X':=X) (X1:=X') (X2:=X0) in H9 as Hws.
       * destruct_eq_atom. simpl in Hws.
@@ -831,8 +1087,8 @@ Proof with eauto; solve_false.
         -- rewrite aworklist_subst_dom_upper with (Γ:=(work_sub ` X0 (typ_arrow A1 A2) ⫤ᵃ X2 ~ᵃ ⬒ ;ᵃ X1 ~ᵃ ⬒ ;ᵃ Γ))...
       * replace ((work_sub ` X0 (typ_arrow ({` X' ᵗ/ₜ X} A1) ({` X' ᵗ/ₜ X} A2)) ⫤ᵃ X2 ~ᵃ ⬒ ;ᵃ X1 ~ᵃ ⬒ ;ᵃ rename_tvar_in_aworklist X' X Γ)) with 
                  (rename_tvar_in_aworklist X' X (work_sub ` X0 (typ_arrow A1 A2) ⫤ᵃ X2 ~ᵃ ⬒ ;ᵃ X1 ~ᵃ ⬒ ;ᵃ Γ)) by (simpl; destruct_eq_atom; auto).
-        apply a_wf_wl_rename_tvar... 
-        destruct_a_wf_wl. repeat (constructor; simpl; auto).
+        apply a_wf_wl_rename_tvar.
+        destruct_a_wf_wl. repeat (constructor; simpl; auto). simpl...
       * solve_notin_rename_tvar; auto.
   - simpl in *. destruct_a_wf_wl.
     destruct (X0 == X); subst;
@@ -866,8 +1122,7 @@ Proof with eauto; solve_false.
     + apply rename_tvar_in_aworklist_bind_same_neq; auto...
     + destruct_a_wf_wl. 
       fold_subst. apply a_mono_typ_false_rename; simpl; eauto.
-    + intros. replace (typ_arrow ({` X' ᵗ/ₜ X} A1) ({` X' ᵗ/ₜ X} A2)) with ({` X' ᵗ/ₜ X} (typ_arrow A1 A2)) in H0...  
-      eapply s_in_subst in H0...
+    + intros. fold_subst. eapply s_in_subst in H0...
     + intros. simpl in *.
       apply worklist_subst_rename_tvar with (X':=X) (X1:=X') (X2:=X0) in H10 as Hws.
       * destruct_eq_atom. simpl in Hws.
@@ -959,22 +1214,16 @@ Proof with eauto; solve_false.
               rewrite_aworklist_rename_rev.
               simpl in Hawlred. destruct_eq_atom. auto.
            ++ eapply aworklist_subst_wf_wl in Hws; simpl in *; eauto 9. 
-              ** repeat (constructor; simpl; auto).
-                 apply a_wf_exp_var_binds_another_cons with (A1:=T)...
-                 rewrite_env (x ~ abind_var_typ T ++ ((X2, ⬒) :: (X1 ~ ⬒)) ++ ⌊ Γ ⌋ᵃ).
-                 apply a_wf_exp_weaken...
+              ** repeat (constructor; simpl; eauto). eapply a_wf_exp_weaken_etvar_twice with (T:=T)...
            ++ rewrite aworklist_subst_dom_upper with (Γ:=(work_check (e ᵉ^ₑ exp_var_f x) ` X2 ⫤ᵃ x ~ᵃ ` X1;ᵃ X2 ~ᵃ ⬒ ;ᵃ X1 ~ᵃ ⬒ ;ᵃ Γ))... 
         -- solve_notin_rename_tvar; auto.
       * replace ((work_check (subst_tvar_in_exp ` X' X e ᵉ^ₑ exp_var_f x) ` X2 ⫤ᵃ x ~ᵃ ` X1;ᵃ X2 ~ᵃ ⬒ ;ᵃ X1 ~ᵃ ⬒ ;ᵃ rename_tvar_in_aworklist X' X Γ)) with 
                 (rename_tvar_in_aworklist X' X (work_check (e ᵉ^ₑ exp_var_f x) ` X2 ⫤ᵃ x ~ᵃ ` X1;ᵃ X2 ~ᵃ ⬒ ;ᵃ X1 ~ᵃ ⬒ ;ᵃ Γ))...
-        apply a_wf_wl_rename_tvar... repeat (constructor; simpl; auto).
-        apply a_wf_exp_var_binds_another_cons with (A1:=T)...
-        rewrite_env (x ~ abind_var_typ T ++ ((X2, ⬒) :: (X1 ~ ⬒)) ++ ⌊ Γ ⌋ᵃ).
-        apply a_wf_exp_weaken...
+        apply a_wf_wl_rename_tvar... repeat (constructor; simpl; eauto).
         simpl. destruct_eq_atom. rewrite subst_tvar_in_exp_open_exp_wrt_exp...
       * simpl. solve_notin_rename_tvar; auto.
     + apply rename_tvar_in_aworklist_bind_same_neq; auto...
-    + intros.
+    + intros. inst_cofinites_with x. inst_cofinites_with X1. inst_cofinites_with X2.  
       apply worklist_subst_rename_tvar with (X':=X) (X1:=X') (X2:=X0) in H11 as Hws.
       destruct_eq_atom.
       * simpl in Hws.
@@ -983,25 +1232,19 @@ Proof with eauto; solve_false.
         replace (exp_var_f x) with (subst_tvar_in_exp (` X') X (exp_var_f x)) in Hws by auto.
         rewrite <- subst_tvar_in_exp_open_exp_wrt_exp in Hws.
         rewrite rename_tvar_in_exp_rev_eq in Hws.
-        -- eapply H7 with (x:=x) in Hws as Hawlred; simpl; auto.
+        -- eapply H7 in Hws as Hawlred; simpl; auto.
            ++ assert (X `notin`(ftvar_in_exp (subst_tvar_in_exp ` X' X e ᵉ^ₑ exp_var_f x))) by (solve_notin_rename_tvar; auto).
               clear Hws. destruct_eq_atom.
               rewrite_aworklist_rename; simpl; auto.
               rewrite_aworklist_rename_rev.
               simpl in Hawlred. destruct_eq_atom. auto.
            ++ eapply aworklist_subst_wf_wl in Hws; simpl; eauto 9.
-              repeat (constructor; simpl; auto). 
-              apply a_wf_exp_var_binds_another_cons with (A1:=T)...
-              rewrite_env (x ~ abind_var_typ T ++ ((X2, ⬒) :: (X1 ~ ⬒)) ++ ⌊ Γ ⌋ᵃ).
-              apply a_wf_exp_weaken...
+              repeat (constructor; simpl; eauto).
            ++ rewrite aworklist_subst_dom_upper with (Γ:=(work_check (e ᵉ^ₑ exp_var_f x) ` X2 ⫤ᵃ x ~ᵃ ` X1;ᵃ X2 ~ᵃ ⬒ ;ᵃ X1 ~ᵃ ⬒ ;ᵃ Γ))...
         -- rewrite ftvar_in_exp_open_exp_wrt_exp_upper; auto.
       * replace ((work_check (subst_tvar_in_exp ` X' X e ᵉ^ₑ exp_var_f x) ` X2 ⫤ᵃ x ~ᵃ ` X1;ᵃ X2 ~ᵃ ⬒ ;ᵃ X1 ~ᵃ ⬒ ;ᵃ rename_tvar_in_aworklist X' X Γ)) with 
                 (rename_tvar_in_aworklist X' X (work_check (e ᵉ^ₑ exp_var_f x) ` X2 ⫤ᵃ x ~ᵃ ` X1;ᵃ X2 ~ᵃ ⬒ ;ᵃ X1 ~ᵃ ⬒ ;ᵃ Γ))...
-        apply a_wf_wl_rename_tvar... repeat (constructor; simpl; auto).
-        apply a_wf_exp_var_binds_another_cons with (A1:=T)...
-        rewrite_env (x ~ abind_var_typ T ++ ((X2, ⬒) :: (X1 ~ ⬒)) ++ ⌊ Γ ⌋ᵃ).
-        apply a_wf_exp_weaken...
+        apply a_wf_wl_rename_tvar... repeat (constructor; simpl; eauto). 
         simpl. destruct_eq_atom. rewrite subst_tvar_in_exp_open_exp_wrt_exp...
       * simpl; solve_notin_rename_tvar; auto.
   - simpl in *.
@@ -1010,7 +1253,7 @@ Proof with eauto; solve_false.
     inst_cofinites_with x.
     rewrite subst_tvar_in_exp_open_exp_wrt_exp in H6...
     apply H6.
-    + repeat (constructor; simpl; auto). 
+    + repeat (constructor; simpl; auto).
       apply a_wf_exp_var_binds_another_cons with (A1:=T)...
     + repeat rewrite ftvar_in_exp_open_exp_wrt_exp_upper...
   - simpl in *.
@@ -1042,12 +1285,9 @@ Proof with eauto; solve_false.
     destruct_eq_atom.
     rewrite subst_tvar_in_exp_open_exp_wrt_exp in H6...
     auto_apply...
-    + repeat (constructor; simpl; auto).
-      * apply a_wf_exp_var_binds_another_cons with (A1:=T)...
-        rewrite_env (x ~ abind_var_typ T ++ ((X2, ⬒) :: (X1 ~ ⬒)) ++ ⌊ Γ ⌋ᵃ).
-        apply a_wf_exp_weaken...
-      * rewrite_env (nil ++ ((X2, ⬒) :: (X1 ~ ⬒)) ++ ⌊ Γ ⌋ᵃ).
-        apply a_wf_conts_weaken...
+    + repeat (constructor; simpl; auto). auto...
+      rewrite_env (nil ++ ((X2, ⬒) :: (X1 ~ ⬒)) ++ ⌊ Γ ⌋ᵃ).
+      apply a_wf_conts_weaken...
   - simpl in *. destruct_a_wf_wl. dependent destruction H0.
     inst_cofinites_for a_wl_red__infabs_all.
     intros. inst_cofinites_with X0.
@@ -1112,49 +1352,36 @@ Proof with eauto; solve_false.
   - simpl in *. destruct_a_wf_wl.
     eapply a_wl_red__inftapp_all.
     rewrite <- subst_tvar_in_typ_open_typ_wrt_typ...
-    auto_apply.
+    auto_apply...
     + repeat (constructor; simpl; auto).
       eapply a_wf_typ_all_open...
-    + auto. 
   - simpl in *.
     eapply apply_conts_rename_tvar with (X:=X) (X':=X') in H2 as Hac...
-    eapply a_wl_red__applys; eauto.
-    auto_apply.
-    eapply a_wf_wl_apply_conts in H0; eauto.
-    auto.
+    eapply a_wl_red__applys...
+    auto_apply...
+    eapply a_wf_wl_apply_conts in H0...
   - simpl in *.
     eapply apply_contd_rename_tvar with (X:=X) (X':=X') in H2 as Hac...
-    eapply a_wl_red__applyd; eauto.
-    auto_apply.
-    eapply a_wf_wl_apply_contd in H0; eauto.
+    eapply a_wl_red__applyd...
+    auto_apply...
+    eapply a_wf_wl_apply_contd in H0... 
 Qed.
 
-Lemma worklist_subst_rename_var : forall Γ x x' X A Γ1 Γ2,
-  ⊢ᵃʷ Γ ->
-  x' `notin` fvar_in_aworklist' Γ ->
-  aworklist_subst Γ X A Γ1 Γ2 ->
-  aworklist_subst (rename_var_in_aworklist x' x Γ) X A (rename_var_in_aworklist x' x Γ1) (rename_var_in_aworklist x' x Γ2).
+
+
+Lemma rename_var_dom_upper : forall Γ x x',
+  dom (awl_to_aenv (rename_var_in_aworklist x' x Γ)) [<=] dom (awl_to_aenv Γ) `union` singleton x'.
 Proof.
-  intros. induction H1; try solve [simpl in *; destruct_a_wf_wl; constructor; auto].
-  simpl. admit.
-  (* apply IHaworklist_subst *)
-Admitted.
+  intros. induction Γ; simpl; try fsetdec.
+  destruct_eq_atom; fsetdec.
+Qed.
 
-Lemma rename_var_in_aworklist_rev_eq : forall x x' Γ,
-  x' `notin` fvar_in_aworklist' Γ ->
-  rename_var_in_aworklist x x' (rename_var_in_aworklist x' x Γ) = Γ.
+
+Lemma fvar_in_aworklist'_awl_app : forall Γ1 Γ2,
+  fvar_in_aworklist' (awl_app Γ2 Γ1) [=] fvar_in_aworklist' Γ2 `union` fvar_in_aworklist' Γ1.
 Proof.
-  induction Γ; simpl in *; auto; intros; destruct_a_wf_wl.
-  - destruct_eq_atom. 
-    + rewrite IHΓ; auto.
-    + rewrite IHΓ; auto.
-  - rewrite IHΓ; auto.
-  - rewrite IHΓ; auto.
-    admit.
-Admitted.
-
-
-
+  induction Γ2; simpl; fsetdec.
+Qed.
 
 Lemma awl_app_rename_var_comm : forall Γ1 Γ2 X X',
   awl_app (rename_var_in_aworklist X' X Γ2) (rename_var_in_aworklist X' X Γ1) =
@@ -1164,11 +1391,102 @@ Proof.
 Qed.
 
 
+
+Lemma worklist_subst_rename_var : forall Γ x x' X A Γ1 Γ2,
+  ⊢ᵃʷ Γ ->
+  x' `notin` fvar_in_aworklist' Γ ->
+  aworklist_subst Γ X A Γ1 Γ2 ->
+  aworklist_subst (rename_var_in_aworklist x' x Γ) X A (rename_var_in_aworklist x' x Γ1) (rename_var_in_aworklist x' x Γ2).
+Proof.
+  intros. induction H1; try solve [simpl in *; destruct_a_wf_wl; constructor; auto].
+  simpl.
+  rewrite <- awl_app_rename_var_comm... simpl.
+  constructor; auto.
+  replace (rename_var_in_aworklist x' x Γ2 ⧺ X ~ᵃ ⬒ ;ᵃ Y ~ᵃ ⬒ ;ᵃ rename_var_in_aworklist x' x Γ1) with (rename_var_in_aworklist x' x (Γ2 ⧺ X ~ᵃ ⬒ ;ᵃ Y ~ᵃ ⬒ ;ᵃ Γ1)).
+  apply IHaworklist_subst. apply a_wf_wl_move_etvar_back... auto.
+  - simpl in *. rewrite fvar_in_aworklist'_awl_app in *. simpl in *. solve_notin.
+  - rewrite <- awl_app_rename_var_comm... simpl. auto.
+Qed.
+
+
+Lemma fvar_in_wf_exp_upper : forall Γ e,
+  a_wf_exp (awl_to_aenv Γ) e ->
+  fvar_in_exp e [<=] dom (awl_to_aenv Γ)
+with fvar_in_wf_body_upper : forall Γ b,
+  a_wf_body (awl_to_aenv Γ) b ->
+  fvar_in_body b [<=] dom (awl_to_aenv Γ).
+Proof.
+  - intros. dependent induction H; try solve [simpl; fsetdec].
+    + simpl. apply binds_In in H... fsetdec.
+    + inst_cofinites_by (L `union` dom (awl_to_aenv Γ) `union` fvar_in_exp e).
+      assert (fvar_in_exp e [<=] fvar_in_exp (e ᵉ^ₑ exp_var_f x)) by apply fvar_in_exp_open_exp_wrt_exp_lower.
+      assert (x ~ abind_var_typ T ++ awl_to_aenv Γ = awl_to_aenv (x ~ᵃ T ;ᵃ Γ)) by (simpl; auto).
+      eapply H1 in H3.
+      simpl in *.
+      fsetdec.
+    + simpl.
+      rewrite IHa_wf_exp1; eauto.
+      rewrite IHa_wf_exp2; eauto.
+      fsetdec.
+    + inst_cofinites_by (L `union` dom (awl_to_aenv Γ) `union` fvar_in_body body5) using_name X.
+      replace (X ~ abind_tvar_empty ++ awl_to_aenv Γ) with (awl_to_aenv (X ~ᵃ □ ;ᵃ Γ)) in H0 by auto.
+      assert (fvar_in_body body5 [<=] fvar_in_body (open_body_wrt_typ body5 ` X)) by apply
+        fvar_in_body_open_body_wrt_typ_lower.
+      apply fvar_in_wf_body_upper in H0.
+      simpl in *.
+      fsetdec.
+    + simpl. rewrite IHa_wf_exp; eauto. fsetdec.
+    + simpl. rewrite IHa_wf_exp; eauto. fsetdec.
+  - intros. destruct b; simpl.
+    + dependent destruction H.
+      rewrite fvar_in_wf_exp_upper; eauto. fsetdec.
+Qed.
+
+
+Lemma fvar_in_wf_conts_upper : forall Γ cs,
+  a_wf_conts (awl_to_aenv Γ) cs ->
+  fvar_in_conts cs [<=] dom (awl_to_aenv Γ)
+with fvar_in_wf_contd_upper : forall Γ cd,
+  a_wf_contd (awl_to_aenv Γ) cd ->
+  fvar_in_contd cd [<=] dom (awl_to_aenv Γ).
+Proof.
+  - intros. intros; dependent induction H;
+    simpl in *;
+    try erewrite fvar_in_wf_exp_upper; eauto;
+    try rewrite IHa_wf_conts; eauto; 
+    try rewrite ftvar_in_wf_contd_upper; eauto;
+    try fsetdec.
+  - intros. intros; dependent induction H;
+    simpl in *;
+    try solve [
+    try destruct_wf_arrow;
+    try erewrite fvar_in_wf_exp_upper; eauto;
+    try rewrite fvar_in_wf_conts_upper; eauto;
+    try rewrite IHa_wf_contd; eauto; 
+    try fsetdec].
+Qed.
+
+Lemma fvar_in_wf_work_upper : forall Γ w,
+  a_wf_work (awl_to_aenv Γ) w ->
+  fvar_in_work w [<=] dom (awl_to_aenv Γ).
+Proof.
+  intros. intros; dependent destruction H;
+    simpl in *;
+    try solve [
+    try repeat destruct_wf_arrow;
+    try erewrite fvar_in_wf_exp_upper; eauto;
+    try rewrite fvar_in_wf_conts_upper; eauto; 
+    try rewrite fvar_in_wf_contd_upper; eauto; try fsetdec].
+Qed.
+
 Lemma fvar_in_aworklist_upper : forall Γ ,
   ⊢ᵃʷ Γ ->
   fvar_in_aworklist' Γ [<=] dom (awl_to_aenv Γ).
 Proof.
-Admitted.
+  intros. induction H; simpl in *; try fsetdec.
+  rewrite fvar_in_wf_work_upper; eauto.
+  fsetdec.
+Qed.
 
 
 Ltac rewrite_fvar_in_aworklist :=
@@ -1176,14 +1494,68 @@ Ltac rewrite_fvar_in_aworklist :=
   | H : context [dom (awl_to_aenv ?Γ)] |- context [fvar_in_aworklist' ?Γ] =>
     rewrite fvar_in_aworklist_upper; auto
   end.
-
-(* Lemma rename_var_in_etvar_list_eq : forall x x' E,
-  rename_var_in_aworklist x x' (etvar_list_to_awl E) = (etvar_list_to_awl E).
+  
+Lemma rename_var_in_aworklist_fresh_eq : forall x x' Γ,
+  x `notin` fvar_in_aworklist' Γ ->
+  rename_var_in_aworklist x' x Γ = Γ.
 Proof.
-  induction E; simpl; auto.
-  rewrite IHE; auto.
-Qed. *)
+  intros. induction Γ; simpl in *; auto.
+  - rewrite IHΓ; auto. 
+    destruct_eq_atom; auto.
+  - rewrite IHΓ; auto.
+  - rewrite IHΓ; auto.
+    rewrite subst_var_in_work_fresh_eq; auto.
+Qed.
 
+
+Lemma subst_tvar_in_exp_rename_var : forall x x' X e A,
+  x' `notin` fvar_in_exp e ->
+  (subst_var_in_exp (exp_var_f x') x (subst_tvar_in_exp A X e)) =
+  (subst_tvar_in_exp A X (subst_var_in_exp (exp_var_f x') x e))
+with subst_tvar_in_body_rename_var : forall x x' X b A,
+   x' `notin` fvar_in_body b ->
+  (subst_var_in_body (exp_var_f x') x (subst_tvar_in_body A X b)) =
+  (subst_tvar_in_body A X (subst_var_in_body (exp_var_f x') x b)).
+Proof with eauto.
+  - intros. induction e; simpl in *; auto...
+    + destruct_eq_atom; simpl; auto. 
+    + rewrite IHe...
+    + rewrite IHe1...
+      rewrite IHe2...
+    + rewrite subst_tvar_in_body_rename_var...
+    + rewrite IHe...
+    + rewrite IHe...
+  - intros. destruct b.
+    simpl in *.
+    erewrite subst_tvar_in_exp_rename_var; auto.
+Qed.
+
+Lemma subst_tvar_in_conts_rename_var : forall x x' X A cs,
+  x' `notin` fvar_in_conts cs ->
+  subst_var_in_conts (exp_var_f x') x ({A ᶜˢ/ₜ X} cs) = {A ᶜˢ/ₜ X} (subst_var_in_conts (exp_var_f x') x cs)
+with subst_tvar_in_contd_rename_var : forall x x' X A cd,
+  x' `notin` fvar_in_contd cd ->
+  subst_var_in_contd (exp_var_f x') x ({A ᶜᵈ/ₜ X} cd) = {A ᶜᵈ/ₜ X} (subst_var_in_contd (exp_var_f x') x cd).
+Proof.
+  - intros. induction cs; simpl in *;
+    try rewrite subst_tvar_in_exp_rename_var; auto;
+    try rewrite IHcs; auto;
+    try rewrite subst_tvar_in_contd_rename_var; auto...
+  - intros. induction cd; simpl in *;
+    try repeat rewrite subst_tvar_in_exp_rename_var; auto;
+    try rewrite IHcd; auto;
+    try rewrite subst_tvar_in_conts_rename_var; auto.
+Qed.
+
+Lemma subst_tvar_in_work_rename_var : forall x x' X w A,
+  x' `notin` fvar_in_work w ->
+  subst_var_in_work (exp_var_f x') x ({A ʷ/ₜ X} w) = {A ʷ/ₜ X} (subst_var_in_work (exp_var_f x') x w).
+Proof.
+  intros. induction w; simpl in *; auto;
+    try rewrite subst_tvar_in_exp_rename_var; auto;
+    try rewrite subst_tvar_in_conts_rename_var; auto;
+    try rewrite subst_tvar_in_contd_rename_var; auto.
+Qed.
 
 Lemma subst_var_in_awl_rename_tvar_comm : forall Γ x x' X A,
   x' `notin` fvar_in_aworklist' Γ ->
@@ -1192,8 +1564,8 @@ Lemma subst_var_in_awl_rename_tvar_comm : forall Γ x x' X A,
 Proof.
   intros. induction Γ; simpl in *; auto; rewrite IHΓ; auto.
   - apply f_equal.
-    admit.
-Admitted.
+    rewrite subst_tvar_in_work_rename_var; auto.
+Qed.
 
 
 Lemma aworklist_subst_fvar_in_aworklist_2 : forall Γ X A Γ1 Γ2,
@@ -1201,8 +1573,8 @@ Lemma aworklist_subst_fvar_in_aworklist_2 : forall Γ X A Γ1 Γ2,
   fvar_in_aworklist' Γ2 [<=] fvar_in_aworklist' Γ.
 Proof.
   intros. induction H; simpl; try fsetdec.
-  admit.
-Admitted.
+  rewrite fvar_in_aworklist'_awl_app in *. fsetdec.
+Qed.
 
 
 Lemma aworklist_subst_fvar_in_aworklist_1 : forall Γ X A Γ1 Γ2,
@@ -1210,9 +1582,60 @@ Lemma aworklist_subst_fvar_in_aworklist_1 : forall Γ X A Γ1 Γ2,
   fvar_in_aworklist' Γ1 [<=] fvar_in_aworklist' Γ.
 Proof.
   intros. induction H; simpl; try fsetdec.
-  admit.
-Admitted.
+  rewrite fvar_in_aworklist'_awl_app in *. fsetdec.
+Qed.
 
+Lemma rename_var_in_aworklist_tvar_bind_same : forall Γ x X' y b,
+  ⊢ᵃʷ Γ ->
+  b = □ \/ b = ■ \/ b = ⬒ ->
+  y `notin` fvar_in_aworklist' Γ ->
+  binds X' b (awl_to_aenv Γ) ->
+  binds X' b (awl_to_aenv (rename_var_in_aworklist y x Γ)).
+Proof with solve_false.
+  intros. induction Γ; simpl in *; auto.
+  - dependent destruction H. destruct_eq_atom.
+    + destruct_binds. destruct H2. inversion H2. destruct H2.  inversion H2. inversion H2.
+      * apply binds_cons; auto.
+    + destruct_binds.
+      * destruct H2. inversion H2. destruct H2. inversion H2. inversion H2.
+      * apply binds_cons; auto. 
+  - dependent destruction H; destruct_binds; auto.
+  - dependent destruction H; eauto.
+Qed.
+
+Lemma rename_var_in_aworklist_var_bind_same : forall Γ x x' y A,
+  ⊢ᵃʷ Γ ->
+  y `notin` fvar_in_aworklist' Γ ->
+  binds x' (abind_var_typ A) (awl_to_aenv Γ) ->
+  binds (if x' == x then y else x') (abind_var_typ A) (awl_to_aenv (rename_var_in_aworklist y x Γ)).
+Proof with solve_false.
+  intros. induction Γ; simpl in *; auto.
+  - dependent destruction H. destruct_eq_atom; destruct_binds; auto.
+  - dependent destruction H; destruct_binds; auto.
+  - dependent destruction H; eauto.
+Qed.
+
+Lemma rename_var_in_aworklist_var_bind_same_eq : forall Γ x y A,
+  ⊢ᵃʷ Γ ->
+  y `notin` fvar_in_aworklist' Γ ->
+  binds x (abind_var_typ A) (awl_to_aenv Γ) ->
+  binds y (abind_var_typ A) (awl_to_aenv (rename_var_in_aworklist y x Γ)).
+Proof with solve_false.
+  intros. eapply rename_var_in_aworklist_var_bind_same with (x':=x) (x:=x) in H1; eauto.
+  destruct_eq_atom. auto.  
+Qed.
+
+
+Lemma rename_var_in_aworklist_var_bind_same_neq : forall Γ x x' y A,
+  ⊢ᵃʷ Γ ->
+  x' <> x ->
+  y `notin` fvar_in_aworklist' Γ ->
+  binds x' (abind_var_typ A) (awl_to_aenv Γ) ->
+  binds x' (abind_var_typ A) (awl_to_aenv (rename_var_in_aworklist y x Γ)).
+Proof with solve_false.
+  intros. eapply rename_var_in_aworklist_var_bind_same with (x':=x') (x:=x) in H1; eauto.
+  destruct_eq_atom. auto.  
+Qed.
 
 Lemma notin_rename_var_in_aworklist : forall x x' Γ,
   x <> x' ->
@@ -1240,9 +1663,57 @@ Proof.
     rewrite rename_var_in_exp_rev_eq; auto.
 Qed.
 
-Lemma apply_cont_rename_var : forall x x' c w A,
-  apply_conts c A w ->
-  apply_conts (subst_var_in_conts (exp_var_f x') x c) A (subst_var_in_work (exp_var_f x') x w).
+
+Lemma rename_var_in_conts_rev_eq : forall x x' cs,
+  x' `notin` fvar_in_conts cs ->
+  subst_var_in_conts (exp_var_f x) x' (subst_var_in_conts (exp_var_f x') x cs) = cs
+with rename_var_in_contd_rev_eq : forall x x' cd,
+  x' `notin` fvar_in_contd cd ->
+  subst_var_in_contd (exp_var_f x) x' (subst_var_in_contd (exp_var_f x') x cd) = cd.
+Proof with auto using rename_var_in_exp_rev_eq.
+  - clear rename_var_in_conts_rev_eq. induction cs; simpl in *; intros;
+      try rewrite rename_var_in_exp_rev_eq; auto;
+      try rewrite IHcs; auto;
+      try rewrite rename_var_in_contd_rev_eq; auto.
+  - clear rename_var_in_contd_rev_eq. induction cd; simpl in *; intros;
+      try rewrite rename_var_in_exp_rev_eq; auto;
+      try rewrite IHcd; auto;
+      try rewrite rename_var_in_conts_rev_eq; auto.
+Qed.
+
+Lemma rename_var_in_work_rev_eq : forall x x' w,
+  x' `notin` fvar_in_work w ->
+  subst_var_in_work (exp_var_f x) x' (subst_var_in_work (exp_var_f x') x w) = w.
+Proof.
+  intros. dependent destruction w; simpl in *;
+    try rewrite rename_var_in_exp_rev_eq; 
+    try rewrite rename_var_in_conts_rev_eq;
+    try rewrite rename_var_in_contd_rev_eq; auto.
+Qed.
+
+Lemma rename_var_in_aworklist_rev_eq : forall x x' Γ,
+  x' `notin` fvar_in_aworklist' Γ ->
+  rename_var_in_aworklist x x' (rename_var_in_aworklist x' x Γ) = Γ.
+Proof.
+  induction Γ; simpl in *; auto; intros; destruct_a_wf_wl.
+  - destruct_eq_atom. 
+    + rewrite IHΓ; auto.
+    + rewrite IHΓ; auto.
+  - rewrite IHΓ; auto.
+  - rewrite IHΓ; auto.
+    rewrite rename_var_in_work_rev_eq; auto.
+Qed.
+
+Lemma apply_conts_rename_var : forall x x' cs w A,
+  apply_conts cs A w ->
+  apply_conts (subst_var_in_conts (exp_var_f x') x cs) A (subst_var_in_work (exp_var_f x') x w).
+Proof.
+  intros. induction H; simpl; try constructor.
+Qed.
+
+Lemma apply_contd_rename_var : forall x x' cd w A B,
+  apply_contd cd A B w ->
+  apply_contd (subst_var_in_contd (exp_var_f x') x cd) A B (subst_var_in_work (exp_var_f x') x w).
 Proof.
   intros. induction H; simpl; try constructor.
 Qed.
@@ -1257,6 +1728,11 @@ Ltac solve_notin_rename_var' :=
     match goal with
     | H1 : x `notin` fvar_in_exp (subst_var_in_exp e1 x e2) |- _ => fail 1
     | _ => assert (x `notin` fvar_in_exp (subst_var_in_exp e1 x e2)) by (apply subst_var_in_exp_fresh_same; auto)
+    end
+  | H : _ |- context [subst_var_in_contd ?cd ?x ?e]  =>
+    match goal with
+    | H1 : x `notin` fvar_in_contd (subst_var_in_contd cd x e) |- _ => fail 1
+    | _ => assert (x `notin` fvar_in_contd (subst_var_in_contd cd x e)) by (apply subst_var_in_contd_fresh_same; auto)
     end
   | H : _ |- context [rename_var_in_aworklist ?x' ?x ?Γ] =>
     (* assert True *)
@@ -1298,6 +1774,153 @@ Ltac rewrite_aworklist_rename_var' :=
 Ltac rewrite_aworklist_rename_var :=
   repeat rewrite_aworklist_rename_var'.
 
+Lemma a_wf_typ_rename_var : forall Γ x x' A,
+  ⊢ᵃʷ Γ ->
+  x' ∉ fvar_in_aworklist' Γ ->
+  ⌊ Γ ⌋ᵃ ᵗ⊢ᵃ A ->
+  ⌊ rename_var_in_aworklist x' x Γ ⌋ᵃ ᵗ⊢ᵃ A.
+Proof.
+  intros. dependent induction H1; try solve [simpl in *; eauto].
+  - constructor. apply rename_var_in_aworklist_tvar_bind_same; auto.
+  - apply a_wf_typ__stvar. apply rename_var_in_aworklist_tvar_bind_same; auto.
+  - apply a_wf_typ__etvar. apply rename_var_in_aworklist_tvar_bind_same; auto.
+  - inst_cofinites_for a_wf_typ__all; intros; inst_cofinites_with X; auto.
+    replace (X ~ □ ++ ⌊ rename_var_in_aworklist x' x Γ ⌋ᵃ ) with (⌊ rename_var_in_aworklist x' x (X ~ᵃ □ ;ᵃ Γ) ⌋ᵃ) by (simpl; auto).
+    apply H1; auto.
+Qed.
+
+
+Lemma a_mono_typ_rename_var : forall Γ x x' T,
+  ⊢ᵃʷ Γ ->
+  x' ∉ fvar_in_aworklist' Γ ->
+  a_mono_typ (⌊ Γ ⌋ᵃ) T ->
+  a_mono_typ (⌊ rename_var_in_aworklist x' x Γ ⌋ᵃ) T.
+Proof.
+  intros. dependent induction H1; try solve [simpl in *; eauto].
+  - constructor. apply rename_var_in_aworklist_tvar_bind_same; auto.
+  - apply a_mono_typ__etvar. apply rename_var_in_aworklist_tvar_bind_same; auto.
+Qed.
+
+
+Lemma lc_exp_subst_var_in_exp : forall e1 e2 x,
+  lc_exp e1 ->
+  lc_exp e2 ->
+  lc_exp (subst_var_in_exp e2 x e1)
+with lc_body_subst_var_in_body : forall b e x,
+  lc_body b ->
+  lc_exp e ->
+  lc_body (subst_var_in_body e x b).
+Proof with eauto using lc_typ_subst.
+  - intros. clear lc_exp_subst_var_in_exp. induction H; simpl...
+    + destruct_eq_atom; auto.
+    + pick fresh x0. apply lc_exp_abs_exists with (x1:=x0). 
+      replace (({e2 ᵉ/ₑ x} e) ᵉ^ₑ exp_var_f x0) with ({e2 ᵉ/ₑ x} (e ᵉ^ₑ exp_var_f x0))...
+      rewrite subst_var_in_exp_open_exp_wrt_exp... simpl; destruct_eq_atom...
+    + pick fresh X0. apply lc_exp_tabs_exists with (X1:=X0).
+      replace (open_body_wrt_typ ({e2 ᵇ/ₑ x} body5) ` X0) with ({e2 ᵇ/ₑ x} (open_body_wrt_typ body5 ` X0))...
+      rewrite subst_var_in_body_open_body_wrt_typ...
+  - intros. clear lc_body_subst_var_in_body. destruct b. 
+      dependent destruction H; simpl...
+Qed.
+
+Lemma a_wf_exp_rename_var : forall Γ x x' e,
+  ⊢ᵃʷ Γ ->
+  x' `notin` fvar_in_aworklist' Γ ->
+  a_wf_exp (⌊ Γ ⌋ᵃ) e ->
+  a_wf_exp (⌊ rename_var_in_aworklist x' x Γ ⌋ᵃ) (subst_var_in_exp (exp_var_f x') x e)
+with a_wf_body_rename_var : forall Γ x x' b,
+  ⊢ᵃʷ Γ ->
+  x' `notin` fvar_in_aworklist' Γ ->
+  a_wf_body (⌊ Γ ⌋ᵃ) b ->
+  a_wf_body (⌊ rename_var_in_aworklist x' x Γ ⌋ᵃ) (subst_var_in_body (exp_var_f x') x b).
+Proof with eauto using a_wf_typ_rename_var.
+  - intros. clear a_wf_exp_rename_var. dependent induction H1; simpl in *...
+    + simpl. destruct_eq_atom.
+      * eapply rename_var_in_aworklist_var_bind_same_eq in H1...
+      * eapply rename_var_in_aworklist_var_bind_same_neq in H1...
+    + inst_cofinites_for a_wf_exp__abs T:=T; intros; inst_cofinites_with x; auto.
+      apply a_wf_typ_rename_var...
+      replace (({exp_var_f x' ᵉ/ₑ x} e) ᵉ^ₑ exp_var_f x0) with ({exp_var_f x' ᵉ/ₑ x} (e ᵉ^ₑ exp_var_f x0)).
+      replace (x0 ~ abind_var_typ T ++ ⌊ rename_var_in_aworklist x' x Γ ⌋ᵃ) with (⌊ rename_var_in_aworklist x' x (x0 ~ᵃ T ;ᵃ Γ) ⌋ᵃ)...
+      * simpl. destruct_eq_atom...
+      * rewrite subst_var_in_exp_open_exp_wrt_exp... simpl. destruct_eq_atom...
+    + inst_cofinites_for a_wf_exp__tabs; intros; inst_cofinites_with X; auto.
+      * destruct body5. simpl.  rewrite open_body_wrt_typ_anno in *.
+        dependent destruction H1. simpl. constructor...
+        replace (({exp_var_f x' ᵉ/ₑ x} e) ᵉ^ₜ ` X) with ({exp_var_f x' ᵉ/ₑ x} ( e ᵉ^ₜ ` X)).
+        apply lc_exp_subst_var_in_exp...
+        rewrite subst_var_in_exp_open_exp_wrt_typ...
+      * replace (open_body_wrt_typ ({exp_var_f x' ᵇ/ₑ x} body5) ` X) with ({exp_var_f x' ᵇ/ₑ x} (open_body_wrt_typ body5 ` X))...
+        replace (X ~ □ ++ ⌊ rename_var_in_aworklist x' x Γ ⌋ᵃ) with (⌊ rename_var_in_aworklist x' x (X ~ᵃ □ ;ᵃ Γ) ⌋ᵃ)...
+        rewrite subst_var_in_body_open_body_wrt_typ...
+  - intros. clear a_wf_body_rename_var. dependent destruction H1. 
+    simpl. constructor...
+Qed.
+
+Lemma a_wf_conts_rename_var : forall Γ x x' cs,
+  ⊢ᵃʷ Γ ->
+  x' `notin` fvar_in_aworklist' Γ ->
+  a_wf_conts (⌊ Γ ⌋ᵃ) cs ->
+  a_wf_conts (⌊ rename_var_in_aworklist x' x Γ ⌋ᵃ) (subst_var_in_conts (exp_var_f x') x cs)
+with a_wf_contd_rename_var : forall Γ x x' cd,
+  ⊢ᵃʷ Γ ->
+  x' `notin` fvar_in_aworklist' Γ ->
+  a_wf_contd (⌊ Γ ⌋ᵃ) cd ->
+  a_wf_contd (⌊ rename_var_in_aworklist x' x Γ ⌋ᵃ) (subst_var_in_contd (exp_var_f x') x cd).
+Proof with eauto using a_wf_typ_rename_var, a_wf_exp_rename_var.
+  - intros. clear a_wf_conts_rename_var. dependent induction H1; simpl...
+  - intros. clear a_wf_contd_rename_var. dependent induction H1; simpl...
+Qed.
+
+
+Lemma a_wf_work_rename_var : forall Γ x x' w,
+  ⊢ᵃʷ Γ ->
+  x' `notin` fvar_in_aworklist' Γ ->
+  a_wf_work (⌊ Γ ⌋ᵃ) w ->
+  a_wf_work (⌊ rename_var_in_aworklist x' x Γ ⌋ᵃ) (subst_var_in_work (exp_var_f x') x w).
+Proof with eauto 10 using a_wf_typ_rename_var, a_wf_exp_rename_var, a_wf_conts_rename_var, a_wf_contd_rename_var.
+  intros. dependent destruction H1; simpl in *...
+Qed.
+
+
+Lemma a_wf_wl_rename_var : forall Γ x x',
+  ⊢ᵃʷ Γ ->
+  x' `notin` dom (awl_to_aenv Γ) ->
+  ⊢ᵃʷ (rename_var_in_aworklist x' x Γ).
+Proof with eauto.
+  intros. induction H; try solve [simpl in *; eauto].
+  - simpl in *. destruct_eq_atom. 
+    + constructor... rewrite rename_var_in_aworklist_fresh_eq; auto.
+      rewrite fvar_in_aworklist_upper; eauto.
+      apply a_wf_typ_rename_var; auto. rewrite fvar_in_aworklist_upper; eauto.
+    + constructor... rewrite rename_var_dom_upper...
+      apply a_wf_typ_rename_var; auto. rewrite fvar_in_aworklist_upper; eauto.
+  - simpl in *. destruct_binds.
+    assert (x' ∉ dom (⌊ Γ ⌋ᵃ)) by auto.
+    apply IHa_wf_wl in H2... constructor... 
+    rewrite rename_var_dom_upper; auto... 
+  - simpl in *. destruct_binds.
+    assert (x' ∉ dom (⌊ Γ ⌋ᵃ)) by auto.
+    apply IHa_wf_wl in H2... constructor... 
+    rewrite rename_var_dom_upper; auto... 
+  - simpl in *. destruct_binds.
+    assert (x' ∉ dom (⌊ Γ ⌋ᵃ)) by auto.
+    apply IHa_wf_wl in H2... constructor... 
+    rewrite rename_var_dom_upper; auto... 
+  - simpl in *. constructor; auto.
+    apply a_wf_work_rename_var...
+    rewrite fvar_in_aworklist_upper; auto... 
+Qed.
+
+
+Ltac create_notin_set_var :=
+  match goal with 
+  | H1 : ⊢ᵃʷ ?Γ , H2 : ?x `notin` dom (⌊ ?Γ ⌋ᵃ) |- _ =>
+    let Hfv := fresh "Hfv" in
+    assert (Hfv: x `notin` fvar_in_aworklist' Γ) by (rewrite fvar_in_aworklist_upper; auto)
+  end.
+
+
 Theorem a_wl_red_rename_var : forall Γ x x',
   ⊢ᵃʷ Γ ->
   x' <> x ->
@@ -1305,84 +1928,103 @@ Theorem a_wl_red_rename_var : forall Γ x x',
   Γ ⟶ᵃʷ⁎⋅ ->
   (rename_var_in_aworklist x' x Γ) ⟶ᵃʷ⁎⋅.
 Proof with eauto.
-  intros. dependent induction H2; try solve [simpl in *; try _apply_IH_a_wl_red; eauto].
+  intros. dependent induction H2; try solve [simpl in *; try _apply_IH_a_wl_red; eauto]; create_notin_set_var.
   - simpl.
-    dependent destruction H.
+    destruct_a_wf_wl. dependent destruction H.
     inst_cofinites_for a_wl_red__sub_alll; auto.
     + intros. simpl in *. inst_cofinites_with X.
       auto_apply; auto.
-      admit. (* wf *)
-  - simpl in *.
+      repeat (constructor; simpl; auto).
+      apply a_wf_typ_tvar_etvar_cons in H0...
+      apply a_wf_typ_weaken_cons...
+  - destruct_a_wf_wl.
+    dependent destruction H.
+    dependent destruction H1.
+    simpl in *.
     inst_cofinites_for a_wl_red__sub_all.
     intros. inst_cofinites_with X...
     auto_apply; auto.
-    admit.  (* wf *)
+    repeat (constructor; simpl; auto).
+    + apply a_wf_typ_tvar_stvar_cons...
+    + apply a_wf_typ_tvar_stvar_cons...
   - simpl in *; destruct_a_wf_wl.
     inst_cofinites_for a_wl_red__sub_arrow1; auto.
-    + admit. (* binds *)
-    + admit. (* mono *)
+    + apply rename_var_in_aworklist_tvar_bind_same... 
+    + intros. eapply a_mono_typ_rename_var with (x':=x) (x:=x') in H0... 
+      * rewrite rename_var_in_aworklist_rev_eq in H0...
+      * apply a_wf_wl_rename_var...
+      * solve_notin_rename_var.
     + intros.
       apply worklist_subst_rename_var with (x:=x') (x':=x) in H10 as Hws; simpl in *.
       * rewrite_aworklist_rename_var_rev.
         apply H8 in Hws as Hawlred; auto.
         -- rewrite_aworklist_rename_var.
-           rewrite_aworklist_rename_var_rev.
-           auto.
-        -- admit. (* wf *)
-        -- admit. (* notin *)
-      * admit.
+           rewrite_aworklist_rename_var_rev...
+        -- eapply aworklist_subst_wf_wl with (Γ:=(work_sub ` X (typ_arrow A1 A2) ⫤ᵃ X2 ~ᵃ ⬒ ;ᵃ X1 ~ᵃ ⬒ ;ᵃ Γ)); simpl; auto...
+           repeat (constructor; simpl; auto).
+        -- rewrite aworklist_subst_dom_upper with (Γ:=(work_sub ` X (typ_arrow A1 A2) ⫤ᵃ X2 ~ᵃ ⬒ ;ᵃ X1 ~ᵃ ⬒ ;ᵃ Γ))...
+      * replace (work_sub ` X (typ_arrow A1 A2) ⫤ᵃ X2 ~ᵃ ⬒ ;ᵃ X1 ~ᵃ ⬒ ;ᵃ rename_var_in_aworklist x' x Γ) with
+          (rename_var_in_aworklist x' x (work_sub ` X (typ_arrow A1 A2) ⫤ᵃ X2 ~ᵃ ⬒ ;ᵃ X1 ~ᵃ ⬒ ;ᵃ Γ)) by (simpl; destruct_eq_atom; auto).
+        apply a_wf_wl_rename_var...
+        repeat (constructor; simpl; auto).
       * solve_notin_rename_var.
   - simpl in *; destruct_a_wf_wl.
     inst_cofinites_for a_wl_red__sub_arrow2; auto.
-    + admit.
-    + admit.
+    + apply rename_var_in_aworklist_tvar_bind_same... 
+    + intros. eapply a_mono_typ_rename_var with (x':=x) (x:=x') in H10... 
+      * rewrite rename_var_in_aworklist_rev_eq in H10...
+      * apply a_wf_wl_rename_var...
+      * solve_notin_rename_var.
     + intros.
       apply worklist_subst_rename_var with (x:=x') (x':=x) in H12 as Hws; simpl in *.
       * rewrite_aworklist_rename_var_rev.
         apply H9 in Hws as Hawlred; auto.
         -- rewrite_aworklist_rename_var.
-           rewrite_aworklist_rename_var_rev.
-           auto.
-        -- admit. (* wf *)
-        -- admit. (* notin *)
-      * admit. (* wf *)
+           rewrite_aworklist_rename_var_rev...
+        -- apply aworklist_subst_wf_wl with (Γ:=(work_sub (typ_arrow A1 A2) ` X ⫤ᵃ X2 ~ᵃ ⬒ ;ᵃ X1 ~ᵃ ⬒ ;ᵃ Γ)); simpl; auto 7.
+           repeat (constructor; simpl; auto).
+        -- rewrite aworklist_subst_dom_upper with (Γ:=(work_sub (typ_arrow A1 A2) ` X ⫤ᵃ X2 ~ᵃ ⬒ ;ᵃ X1 ~ᵃ ⬒ ;ᵃ Γ))...
+      * replace (work_sub (typ_arrow A1 A2) ` X ⫤ᵃ X2 ~ᵃ ⬒ ;ᵃ X1 ~ᵃ ⬒ ;ᵃ rename_var_in_aworklist x' x Γ) with
+          (rename_var_in_aworklist x' x (work_sub (typ_arrow A1 A2) ` X ⫤ᵃ X2 ~ᵃ ⬒ ;ᵃ X1 ~ᵃ ⬒ ;ᵃ Γ)) by (simpl; destruct_eq_atom; auto).
+        apply a_wf_wl_rename_var...
+        repeat (constructor; simpl; auto).
       * solve_notin_rename_var.
   - simpl in *; destruct_a_wf_wl.
     eapply a_wl_red__sub_etvarmono1 with (Γ1:=(rename_var_in_aworklist x' x Γ1))
       (Γ2:=(rename_var_in_aworklist x' x Γ2)); auto.
-    + admit. (* binds *)
-    + admit. (* mono *)
+    + apply rename_var_in_aworklist_tvar_bind_same... 
+    + apply a_mono_typ_rename_var with (x':=x') (x:=x) in H5...
     + apply worklist_subst_rename_var with (x:=x) (x':=x') in H7 as Hws; eauto.
-      * rewrite fvar_in_aworklist_upper; auto.
     + rewrite_aworklist_rename_var.
-      rewrite_aworklist_rename_var_rev.
+      rewrite_aworklist_rename_var_rev...
       auto_apply; auto.
-      * admit. (* wf *)
-      * admit. (* notin *)
+      * eapply aworklist_subst_wf_wl...
+      * erewrite aworklist_subst_dom_upper...
   - simpl in *; destruct_a_wf_wl.
     eapply a_wl_red__sub_etvarmono2 with (Γ1:=(rename_var_in_aworklist x' x Γ1))
       (Γ2:=(rename_var_in_aworklist x' x Γ2)); auto.
-    + admit. (* binds *)
-    + admit. (* mono *)
+    + apply rename_var_in_aworklist_tvar_bind_same... 
+    + apply a_mono_typ_rename_var with (x':=x') (x:=x) in H5...
     + apply worklist_subst_rename_var with (x:=x) (x':=x') in H7 as Hws; eauto.
-      * rewrite fvar_in_aworklist_upper; auto.
     + rewrite_aworklist_rename_var.
       rewrite_aworklist_rename_var_rev.
       auto_apply.
-      * admit. (* wf *)
-      * admit. (* notin *)
-  - simpl in *.
+      * eapply aworklist_subst_wf_wl...
+      * erewrite aworklist_subst_dom_upper...
+  - destruct_a_wf_wl. simpl in *. 
     inst_cofinites_for a_wl_red__chk_absarrow. intros.
     inst_cofinites_with x0.
     destruct_eq_atom.
     rewrite subst_var_in_exp_open_exp_wrt_exp in *... simpl in *.
     destruct_eq_atom.
     auto_apply...
-    admit. (* wf *)
+    repeat (constructor; simpl; auto)...
+    + apply a_wf_exp_var_binds_another_cons with (A1:=T)...
+    + apply a_wf_typ_weaken_cons...
   - simpl in *; destruct_a_wf_wl.
     inst_cofinites_for a_wl_red__chk_absetvar.
-    + admit. (* binds *)
-    + intros.
+    + apply rename_var_in_aworklist_tvar_bind_same... 
+    + intros. inst_cofinites_with x0. inst_cofinites_with X1. inst_cofinites_with X2.
       apply worklist_subst_rename_var with (x:=x') (x':=x) in H11 as Hws.
       simpl in Hws. destruct_eq_atom.
       rewrite_aworklist_rename_var_rev.
@@ -1393,37 +2035,49 @@ Proof with eauto.
         rewrite rename_var_in_exp_rev_eq in Hws.
         -- apply H7 in Hws; auto.
            ++ rewrite_aworklist_rename_var.
-              rewrite_aworklist_rename_var_rev.
-              auto.
-           ++ admit. (* wf *)
-           ++ admit. (* notin *)
-        -- admit. (* notin *)
-      * admit. (* wf *)
+              rewrite_aworklist_rename_var_rev...
+           ++ apply aworklist_subst_wf_wl with (Γ:=(work_check (e ᵉ^ₑ exp_var_f x0) ` X2 ⫤ᵃ x0 ~ᵃ ` X1;ᵃ X2 ~ᵃ ⬒ ;ᵃ X1 ~ᵃ ⬒ ;ᵃ Γ)); simpl; auto 7... 
+              repeat (constructor; simpl; auto)... apply a_wf_exp_weaken_etvar_twice with (T:=T)...
+           ++ rewrite aworklist_subst_dom_upper with (Γ:=(work_check (e ᵉ^ₑ exp_var_f x0) ` X2 ⫤ᵃ x0 ~ᵃ ` X1;ᵃ X2 ~ᵃ ⬒ ;ᵃ X1 ~ᵃ ⬒ ;ᵃ Γ))...
+        -- solve_notin_rename_var.
+      * replace ((work_check (({exp_var_f x' ᵉ/ₑ x} e) ᵉ^ₑ exp_var_f x0) ` X2 ⫤ᵃ x0 ~ᵃ ` X1;ᵃ X2 ~ᵃ ⬒ ;ᵃ X1 ~ᵃ ⬒ ;ᵃ rename_var_in_aworklist x' x Γ)) with 
+                (rename_var_in_aworklist x' x (work_check (e ᵉ^ₑ exp_var_f x0) ` X2 ⫤ᵃ x0 ~ᵃ ` X1;ᵃ X2 ~ᵃ ⬒ ;ᵃ X1 ~ᵃ ⬒ ;ᵃ Γ))...
+        apply a_wf_wl_rename_var...
+        repeat (constructor; simpl; auto)...
+        simpl. rewrite subst_var_in_exp_open_exp_wrt_exp; simpl; destruct_eq_atom...
       * simpl.
         rewrite fvar_in_exp_open_exp_wrt_exp_upper.
         assert (x `notin` fvar_in_exp ({exp_var_f x' ᵉ/ₑ x} e)) by (apply subst_var_in_exp_fresh_same; auto).
         solve_notin_rename_var.
-  - simpl in *.
+  - destruct_a_wf_wl. simpl in *.
     inst_cofinites_for a_wl_red__chk_abstop. intros.
     inst_cofinites_with x0.
-    destruct_eq_atom.
+    destruct_eq_atom. 
     rewrite subst_var_in_exp_open_exp_wrt_exp in *... simpl in *.
     destruct_eq_atom.
     auto_apply...
-    admit. (* wf *)
+    repeat (constructor; simpl; auto).
+    eapply a_wf_exp_var_binds_another_cons with (A1:=T); eauto.
   - simpl in *.
     destruct (x0 == x); subst; apply a_wl_red__inf_var with (A:=A).
-    + admit.
-    + auto_apply; auto. admit.
-    + admit.
-    + auto_apply; auto. admit.
-  - simpl in *.
-    inst_cofinites_for  a_wl_red__inf_tabs...
+    + destruct_a_wf_wl... apply rename_var_in_aworklist_var_bind_same_eq...  
+    + auto_apply; auto. destruct_a_wf_wl. unify_binds. apply a_wf_wl_wf_bind_typ in H...
+    + destruct_a_wf_wl... apply rename_var_in_aworklist_var_bind_same_neq...  
+    + auto_apply; auto. destruct_a_wf_wl. unify_binds. apply a_wf_wl_wf_bind_typ in H...
+  - destruct_a_wf_wl. simpl in *.
+    inst_cofinites_for a_wl_red__inf_tabs...
     intros. inst_cofinites_with X.
     rewrite subst_var_in_exp_open_exp_wrt_typ in *...
+    rewrite open_body_wrt_typ_anno in *.
     auto_apply...
-    admit. (* wf *)
-  - simpl in *.
+    dependent destruction H0. dependent destruction H.
+    repeat (constructor; simpl; auto).
+    + inst_cofinites_for a_wf_typ__all; intros.
+      * apply s_in_rename with (Y:=X0) in H0...
+        rewrite subst_tvar_in_typ_open_typ_wrt_typ_tvar2 in H0...
+      * apply a_wf_typ_rename_tvar_cons with (Y:=X0) in H1...
+        rewrite subst_tvar_in_typ_open_typ_wrt_typ_tvar2 in H1...
+  - destruct_a_wf_wl. simpl in *.
     inst_cofinites_for a_wl_red__inf_abs_mono.
     intros.
     destruct_eq_atom.
@@ -1432,24 +2086,50 @@ Proof with eauto.
     rewrite subst_var_in_exp_open_exp_wrt_exp in *; auto; simpl in *.
     destruct_eq_atom.
     auto_apply; auto.
-    admit. (* wf *)
-  - simpl in *.
+    repeat (constructor; simpl; auto)...
+    apply a_wf_exp_weaken_etvar_twice with (T:=T)...
+    apply a_wf_conts_weaken_cons...  apply a_wf_conts_weaken_cons...
+  - destruct_a_wf_wl. dependent destruction H. simpl in *.
     inst_cofinites_for a_wl_red__infabs_all.
     intros. inst_cofinites_with X.
     auto_apply; auto.
-    admit. (* wf *)
-  - simpl in *.
+    repeat (constructor; simpl; auto).
+    apply a_wf_typ_tvar_etvar_cons...
+    apply a_wf_contd_weaken_cons...
+  -  destruct_a_wf_wl. simpl in *.
     inst_cofinites_for a_wl_red__infabs_etvar; auto.
-    + admit. (* binds *)
-    + intros. admit.
-  - simpl in *.
+    + apply rename_var_in_aworklist_tvar_bind_same...
+    + intros. apply worklist_subst_rename_var with (x:=x') (x':=x) in H9 as Hws...
+      * simpl in Hws. destruct_eq_atom.
+        rewrite rename_var_in_aworklist_rev_eq in Hws...
+        rewrite rename_var_in_contd_rev_eq in Hws...
+        apply H6 in Hws as Hawlred; simpl; auto.
+        -- rewrite_aworklist_rename_var.
+           rewrite_aworklist_rename_var_rev...
+        -- destruct_a_wf_wl. 
+           apply aworklist_subst_wf_wl with (Γ:=(work_infabs (typ_arrow ` X1 ` X2) cd ⫤ᵃ X2 ~ᵃ ⬒ ;ᵃ X1 ~ᵃ ⬒ ;ᵃ Γ)); simpl; auto.
+           repeat (constructor; simpl; auto).
+           apply a_wf_contd_weaken_cons... apply a_wf_contd_weaken_cons...
+        -- rewrite aworklist_subst_dom_upper with (Γ:=(work_infabs (typ_arrow ` X1 ` X2) cd ⫤ᵃ X2 ~ᵃ ⬒ ;ᵃ X1 ~ᵃ ⬒ ;ᵃ Γ))...
+      * replace (work_infabs (typ_arrow ` X1 ` X2) (subst_var_in_contd (exp_var_f x') x cd) ⫤ᵃ X2 ~ᵃ ⬒ ;ᵃ X1 ~ᵃ ⬒ ;ᵃ rename_var_in_aworklist x' x Γ) with 
+                 (rename_var_in_aworklist x' x (work_infabs (typ_arrow ` X1 ` X2) cd ⫤ᵃ X2 ~ᵃ ⬒ ;ᵃ X1 ~ᵃ ⬒ ;ᵃ Γ)) by (simpl; destruct_eq_atom; auto).
+        apply a_wf_wl_rename_var...
+        repeat (constructor; simpl; auto). 
+        apply a_wf_contd_weaken_cons... apply a_wf_contd_weaken_cons...
+      * solve_notin_rename_var. 
+  - destruct_a_wf_wl. 
     eapply a_wl_red__inftapp_all.
     auto_apply; auto.
-    admit. (* wf *)
+    repeat (constructor; simpl; auto).
+    apply a_wf_typ_all_open...
   - simpl in *.
-    eapply apply_cont_rename_var with (x':=x') (x:=x) in H2 as Hac.
+    eapply apply_conts_rename_var with (x':=x') (x:=x) in H2 as Hac.
     econstructor; eauto.
     auto_apply...
     eapply a_wf_wl_apply_conts; eauto.
-  - admit. (* *, should be same as above *)
-Admitted.
+  - simpl in *.
+    eapply apply_contd_rename_var with (x':=x') (x:=x) in H2 as Hac.
+    econstructor; eauto.
+    auto_apply...
+    eapply a_wf_wl_apply_contd; eauto.
+Qed.
