proof/old_system/_.v
@@ -10,7 +10,7 @@ Require Import uni.algo_worklist.def_extra.
 
 Require Import uni.algo_worklist.prop_soundness.
 Require Import uni.algo_worklist.prop_completeness.
-Require Import uni.algo_worklist.prop_decidability.
+(* Require Import uni.algo_worklist.prop_decidability. *)
 
 (* Prop of decl system *)
 Print Assumptions d_chk_inf_subsumption.
@@ -20,4 +20,5 @@ Print Assumptions d_wl_red_complete.
 Print Assumptions d_wl_red_sound.
 
 (* Prop of algo worklist system *)
+Print Assumptions a_wl_red_soundness.
 Print Assumptions a_wl_red_completeness.
